Working on substitution

proof/Simple/Env.v
@@ -14,10 +14,21 @@ Implicit Arguments some [[a]].
 Inductive env (A: Type) : Type :=
  | empty  : env A
  | snoc   : env A -> A -> env A.
+Hint Constructors env.
 
 Implicit Arguments empty [A].
 Implicit Arguments snoc  [A].
-Infix ":>" := snoc (at level 61, left associativity).
+
+
+Fixpoint cons   {A: Type} (x: A) (e: env A) : env A :=
+ match e with
+ | empty      => snoc empty x
+ | snoc e' y  => snoc (cons x e') y
+ end.
+
+Implicit Arguments cons  [A].
+Infix ":>" := snoc (at level 61, left  associativity).
+Infix "<:" := cons (at level 62, right associativity).
 
 
 Fixpoint length {A: Type} (e: env A) : nat :=
@@ -25,5 +36,35 @@ Fixpoint length {A: Type} (e: env A) : nat :=
  | empty      => 0
  | snoc e' x  => S (length e')
  end.
+Hint Unfold length.
+
+
+Fixpoint get {A: Type} (e: env A) (i: nat) : option A :=
+ match e, i with
+ | snoc _ T,  O    => some T
+ | snoc xs _, S i' => get  xs i'
+ | _, _            => none
+ end.
+
+
+Fixpoint take {A: Type} (n: nat) (e: env A) : env A :=
+ match n, e with
+ | O,   _       => empty
+ | S n, e' :> T => take n e' :> T
+ | S n, empty   => empty
+ end.
+Hint Unfold take.
+
+
+(* Lemmas ***********************************************************)
+Lemma env_snoc_cons
+ :  forall A (e: env A) (x: A) (y: A)
+ ,  ((x <: e) :> y) = (x <: (e :> y)).
+Proof.
+ intros. destruct e.
+ simpl. auto.
+ simpl. auto.
+Qed.
+
 
 
